Wrote up code flattening

07ByteCode/CodeFlattening.thy
@@ -24,12 +24,66 @@ fun flatten_code' :: "nat \<Rightarrow> code\<^sub>e list \<Rightarrow> code\<^s
 definition flatten_code :: "code\<^sub>e list \<Rightarrow> code\<^sub>b list" where
   "flatten_code \<C> \<equiv> flatten_code' 0 \<C>"
 
+lemma properly_terminated_flatten' [simp]: "properly_terminated\<^sub>e \<C> \<Longrightarrow> 
+    properly_terminated\<^sub>b (flatten_code' p \<C> @ \<C>')"
+  by (induction p \<C> arbitrary: \<C>' rule: flatten_code'.induct) 
+     (auto simp add: Let_def split: if_splits)
+
+lemma properly_terminated_flatten [simp]: "properly_terminated\<^sub>e \<C> \<Longrightarrow> 
+  properly_terminated\<^sub>b (flatten_code \<C>)"
+proof (unfold flatten_code_def)
+  assume "properly_terminated\<^sub>e \<C>"
+  hence "properly_terminated\<^sub>b (flatten_code' 0 \<C> @ [])" by (metis properly_terminated_flatten')
+  thus "properly_terminated\<^sub>b (flatten_code' 0 \<C>)" by simp
+qed
+
+text \<open>We also define a function to directly calculate the length of a flattened piece of code. (The
+reason we do not use \<open>length (flatten_code' p \<C>)\<close> is that the p argument is irrelevant to the 
+length.)\<close>
+
+primrec code_size :: "code\<^sub>e \<Rightarrow> nat"
+    and code_list_size :: "code\<^sub>e list \<Rightarrow> nat" where
+  "code_size (Lookup\<^sub>e x) = 1"
+| "code_size (PushCon\<^sub>e n) = 1"
+| "code_size (PushLam\<^sub>e \<C>) = Suc (code_list_size \<C>)"
+| "code_size Apply\<^sub>e = 1"
+| "code_size Return\<^sub>e = 1"
+| "code_size Jump\<^sub>e = 1"
+| "code_list_size [] = 0"
+| "code_list_size (op # \<C>) = code_size op + code_list_size \<C>"
+
+lemma length_flatten' [simp]: "length (flatten_code' p \<C>) = code_list_size \<C>"
+  by (induction p \<C> rule: flatten_code'.induct) simp_all
+
+lemma length_flatten [simp]: "length (flatten_code \<C>) = code_list_size \<C>"
+  by (simp add: flatten_code_def)
+
+lemma code_size_nz [simp]: "0 < code_size \<C>"
+  by (induction \<C>) simp_all
+
+lemma code_list_size_empty [simp]: "(code_list_size \<C> = 0) = (\<C> = [])"
+  by (induction \<C>) simp_all
+
+lemma index_into_append [simp]: "lookup (flatten_code' m \<C> @ \<C>') (code_list_size \<C> + n) = 
+    lookup \<C>' n"
+  by (metis length_flatten' lookup_append_snd)
+
+lemma index_into_flatten [simp]: "lookup (flatten_code' n \<C> @ op # \<C>') (code_list_size \<C>) = 
+  Some op"
+proof -
+  have "lookup (flatten_code' n \<C> @ op # \<C>') (code_list_size \<C> + 0) = lookup (op # \<C>') 0" 
+    by (metis index_into_append)
+  thus ?thesis by simp
+qed
+
 text \<open>One might think that, like previous compilation passes, we could simply map \<open>flatten_code\<close> up
 the levels of the state and produce a compiled state. Unfortunately, we cannot. Once evaluation 
 begins, the code stored in the tree-code stack could come from all over the codebase, and there is 
 no guarantee that \<open>flatten_code\<close> would assign the right internal addresses. The structure of the 
 code would be the same, of course, but rather than get bogged down in trying to define an 
-"alpha-equivalence for code pointers" we cut to the chase and define a code-unflattening function.\<close>
+"alpha-equivalence for code pointers" we cut to the chase and define a code-unflattening function. 
+Note the importance for termination of each nested code pointer being less than the address of its 
+operation.\<close>
 
 fun unflatten_code :: "code\<^sub>b list \<Rightarrow> nat \<Rightarrow> code\<^sub>e list" where
   "unflatten_code \<C> 0 = []"
@@ -59,6 +113,40 @@ abbreviation unflatten_stack :: "code\<^sub>b list \<Rightarrow> (closure\<^sub>
 primrec unflatten_state :: "code\<^sub>b list \<Rightarrow> state\<^sub>b \<Rightarrow> state\<^sub>e" where
   "unflatten_state \<C> (S\<^sub>b \<V> s) = S\<^sub>e (unflatten_values \<C> \<V>) (unflatten_stack \<C> s)"
 
+lemma unflatten_front [simp]: "p \<le> length \<C> \<Longrightarrow> unflatten_code (\<C> @ \<C>') p = unflatten_code \<C> p"
+  by (induction \<C> p rule: unflatten_code.induct) (simp_all split: option.splits code\<^sub>b.splits) 
+
+lemma unflatten_flatten' [simp]: "properly_terminated\<^sub>e \<C> \<Longrightarrow> 
+  unflatten_code (\<C>' @ flatten_code' (length \<C>') \<C> @ \<C>'') (length \<C>' + code_list_size \<C>) = \<C>"
+proof (induction "length \<C>'" \<C> arbitrary: \<C>' \<C>'' rule: flatten_code'.induct)
+  case (4 \<C>\<^sub>2 \<C>\<^sub>1)
+  let ?pc = "length \<C>' + code_list_size \<C>\<^sub>2"
+  let ?code' = "\<C>' @ flatten_code' (length \<C>') \<C>\<^sub>2 @ []"
+  let ?code = "?code' @ flatten_code' ?pc \<C>\<^sub>1 @ PushLam\<^sub>b ?pc # \<C>''"
+  have X: "length \<C>' + length (flatten_code' (length \<C>') \<C>\<^sub>2) = length ?code'" by simp
+  from 4 have "properly_terminated\<^sub>e \<C>\<^sub>1" by simp
+  with 4 X have "unflatten_code (?code' @ flatten_code' (length ?code') \<C>\<^sub>1 @
+    PushLam\<^sub>b (length \<C>' + length (flatten_code' (length \<C>') \<C>\<^sub>2)) # \<C>'')
+      (length ?code' + code_list_size \<C>\<^sub>1) = \<C>\<^sub>1" by blast
+  hence "unflatten_code ?code (length \<C>' + code_list_size \<C>\<^sub>2 + code_list_size \<C>\<^sub>1) = \<C>\<^sub>1" by simp
+  hence X: "unflatten_code ?code (length \<C>' + (code_list_size \<C>\<^sub>2 + code_list_size \<C>\<^sub>1)) = \<C>\<^sub>1" 
+    by (metis add.assoc)
+  from 4 have "properly_terminated\<^sub>e \<C>\<^sub>2" by simp
+  with 4 have "unflatten_code ?code' (length \<C>' + code_list_size \<C>\<^sub>2) = \<C>\<^sub>2" by blast
+  moreover have "?pc \<le> length ?code'" by simp
+  ultimately have Z: "unflatten_code ?code ?pc = \<C>\<^sub>2" by (metis unflatten_front)
+  with X Z show ?case by simp
+qed simp_all
+
+lemma unflatten_flatten [simp]: "properly_terminated\<^sub>e \<C> \<Longrightarrow> 
+  unflatten_code (flatten_code \<C>) (code_list_size \<C>) = \<C>"
+proof -
+  assume "properly_terminated\<^sub>e \<C>"
+  hence "unflatten_code ([] @ flatten_code' (length []) \<C> @ []) 
+    (length [] + code_list_size \<C>) = \<C>" by (metis unflatten_flatten' list.size(3))
+  thus ?thesis by (simp add: flatten_code_def)
+qed
+
 text \<open>We have noted already that all the pointers in the codebase should go towards smaller 
 addresses. We now define some predicates to assert this formally:\<close>
 
@@ -81,450 +169,361 @@ fun orderly_stack :: "(closure\<^sub>b list \<times> nat) list \<Rightarrow> nat
     (p < n \<and> list_all (orderly_closure n) \<Delta> \<and> orderly_stack s n)"
 
 primrec orderly_state :: "code\<^sub>b list \<Rightarrow> state\<^sub>b \<Rightarrow> bool" where
-  "orderly_state cd (S\<^sub>b vs sfs) = (orderly_code cd 0 \<and> properly_terminated\<^sub>b cd \<and> 
-    orderly_stack sfs (length cd) \<and> list_all (orderly_closure (length cd)) vs)"
+  "orderly_state \<C> (S\<^sub>b \<V> s) = (orderly_code \<C> 0 \<and> properly_terminated\<^sub>b \<C> \<and> 
+    orderly_stack s (length \<C>) \<and> list_all (orderly_closure (length \<C>)) \<V>)"
 
-primrec code_size :: "code\<^sub>e \<Rightarrow> nat"
-    and code_list_size :: "code\<^sub>e list \<Rightarrow> nat" where
-  "code_size (Lookup\<^sub>e x) = 1"
-| "code_size (PushCon\<^sub>e n) = 1"
-| "code_size (PushLam\<^sub>e \<C>) = Suc (code_list_size \<C>)"
-| "code_size Apply\<^sub>e = 1"
-| "code_size Return\<^sub>e = 1"
-| "code_size Jump\<^sub>e = 1"
-| "code_list_size [] = 0"
-| "code_list_size (op # \<C>) = code_size op + code_list_size \<C>"
+lemma orderly_append [simp]: "orderly_code (\<C> @ \<C>') n = 
+    (orderly_code \<C> n \<and> orderly_code \<C>' (length \<C> + n))"
+  by (induction \<C> arbitrary: n) simp_all
 
-lemma flatten_length [simp]: "length (flatten_code' lib cd) = code_list_size cd"
-  by (induction lib cd rule: flatten_code'.induct) simp_all
+lemma orderly_flatten' [simp]: "p \<le> n \<Longrightarrow> properly_terminated\<^sub>e \<C> \<Longrightarrow> 
+    orderly_code (flatten_code' p \<C>) n"
+  by (induction p \<C> arbitrary: n rule: flatten_code'.induct) auto
 
-lemma [simp]: "length (flatten_code cd) = code_list_size cd"
+lemma orderly_flatten [simp]: "properly_terminated\<^sub>e \<C> \<Longrightarrow> orderly_code (flatten_code \<C>) 0"
   by (simp add: flatten_code_def)
 
-lemma [simp]: "0 < code_size cd"
-  by (induction cd) simp_all
-
-lemma [simp]: "(code_list_size cd = 0) = (cd = [])"
-  by (induction cd) simp_all
-
-lemma [simp]: "(flatten_code' lib cd = []) = (cd = [])"
-  by (induction lib cd rule: flatten_code'.induct) simp_all
-
-lemma [simp]: "(flatten_code cd = []) = (cd = [])"
-  by (simp add: flatten_code_def)
-
-lemma [simp]: "cd \<noteq> [] \<Longrightarrow> properly_terminated\<^sub>b (cd @ cd') = properly_terminated\<^sub>b cd"
-  by (induction cd) simp_all
-
-lemma return_terminated_flatten' [simp]: "properly_terminated\<^sub>e cd \<Longrightarrow> 
-    properly_terminated\<^sub>b (flatten_code' lib cd @ cd')"
-  by (induction lib cd arbitrary: cd' rule: flatten_code'.induct) (auto split: if_splits)
-
-lemma [simp]: "properly_terminated\<^sub>e cd \<Longrightarrow> properly_terminated\<^sub>b (flatten_code cd)"
-proof (unfold flatten_code_def)
-  assume "properly_terminated\<^sub>e cd"
-  hence "properly_terminated\<^sub>b (flatten_code' 0 cd @ [])" by (metis return_terminated_flatten')
-  thus "properly_terminated\<^sub>b (flatten_code' 0 cd)" by simp
-qed
-
-lemma [simp]: "orderly_op x op \<Longrightarrow> orderly_op (Suc x) op"
-  by (induction op) simp_all
-
-lemma [simp]: "orderly_op (x + n) op \<Longrightarrow> orderly_op (x + (m + n)) op"
-  by (induction op) simp_all
-
-lemma [simp]: "orderly_code (cd @ cd') n = (orderly_code cd n \<and> orderly_code cd' (length cd + n))"
-  by (induction cd arbitrary: n) simp_all
-
-lemma [simp]: "lib \<le> n \<Longrightarrow> properly_terminated\<^sub>e cd \<Longrightarrow> orderly_code (flatten_code' lib cd) n"
-  by (induction lib cd arbitrary: n rule: flatten_code'.induct) auto
-
-lemma [simp]: "properly_terminated\<^sub>e cdr \<Longrightarrow> orderly_code (flatten_code cdr) 0"
-  by (simp add: flatten_code_def)
-
-lemma [simp]: "x > 0 \<Longrightarrow> orderly_stack [([], x)] x"
+lemma orderly_empty_frame [simp]: "x > 0 \<Longrightarrow> orderly_stack [([], x)] x"
   by (cases x) simp_all
 
-lemma orderly_length_flatten [simp]: "cdr \<noteq> [] \<Longrightarrow> 
-    orderly_stack [([], length (flatten_code cdr))] (length (flatten_code cdr))"
-  by (cases cdr) simp_all
+lemma orderly_length_flatten [simp]: "\<C> \<noteq> [] \<Longrightarrow> 
+    orderly_stack [([], length (flatten_code \<C>))] (length (flatten_code \<C>))"
+  by (cases \<C>) simp_all
 
-lemma [simp]: "cdr \<noteq> [] \<Longrightarrow> orderly_stack [([], code_list_size cdr)] (code_list_size cdr)"
+lemma orderly_code_size [simp]: "\<C> \<noteq> [] \<Longrightarrow> 
+    orderly_stack [([], code_list_size \<C>)] (code_list_size \<C>)"
 proof -
-  assume "cdr \<noteq> []" 
-  hence "orderly_stack [([], length (flatten_code cdr))] (length (flatten_code cdr))" 
+  assume "\<C> \<noteq> []" 
+  hence "orderly_stack [([], length (flatten_code \<C>))] (length (flatten_code \<C>))" 
     by (metis orderly_length_flatten)
   thus ?thesis by simp
 qed
- 
-lemma [simp]: "lookup vs x = Some v \<Longrightarrow> list_all (orderly_closure n) vs \<Longrightarrow> orderly_closure n v"
-  by auto
 
-lemma pushlam_ordered [simp]: "lookup cd x = Some (PushLam\<^sub>b pc) \<Longrightarrow> orderly_code cd n \<Longrightarrow> 
-    x < length cd \<Longrightarrow> 0 < pc \<and> pc \<le> length cd + n"
-  by (induction cd x arbitrary: n rule: lookup.induct) fastforce+
+lemma pushlam_ordered' [simp]: "lookup \<C> x = Some (PushLam\<^sub>b p) \<Longrightarrow> orderly_code \<C> n \<Longrightarrow> 
+    x < length \<C> \<Longrightarrow> 0 < p \<and> p \<le> length \<C> + n"
+  by (induction \<C> x arbitrary: n rule: lookup.induct) fastforce+
 
-lemma [simp]: "lookup cd x = Some (PushLam\<^sub>b pc) \<Longrightarrow> orderly_code cd 0 \<Longrightarrow> x < length cd \<Longrightarrow> 
-    0 < pc \<and> pc \<le> length cd"
-  using pushlam_ordered by fastforce
+lemma pushlam_ordered [simp]: "lookup \<C> x = Some (PushLam\<^sub>b p) \<Longrightarrow> orderly_code \<C> 0 \<Longrightarrow> 
+    x < length \<C> \<Longrightarrow> 0 < p \<and> p \<le> length \<C>"
+  using pushlam_ordered' by fastforce
 
-lemma index_into_append [simp]: "lookup (flatten_code' lib cd @ cd') (code_list_size cd + n) = 
-    lookup cd' n"
-  by (metis flatten_length lookup_append_snd)
+lemma orderly_lam' [simp]: "lookup \<C> p = Some (PushLam\<^sub>b p') \<Longrightarrow> orderly_code \<C> n \<Longrightarrow> p' \<le> p + n"
+  by (induction \<C> p arbitrary: n rule: lookup.induct) fastforce+
 
-lemma [simp]: "lookup (flatten_code' lib cd @ op # acc) (code_list_size cd) = Some op"
-proof -
-  have "lookup (flatten_code' lib cd @ op # acc) (code_list_size cd + 0) = lookup (op # acc) 0" 
-    by (metis index_into_append)
-  thus ?thesis by simp
-qed
+lemma orderly_lam [simp]: "lookup \<C> p = Some (PushLam\<^sub>b p') \<Longrightarrow> orderly_code \<C> 0 \<Longrightarrow> p' \<le> p"
+  using orderly_lam' by fastforce
 
-lemma unflatten_front [simp]: "pc \<le> length cd \<Longrightarrow> 
-    unflatten_code (cd @ cd') pc = unflatten_code cd pc"
-  by (induction cd pc rule: unflatten_code.induct) (simp_all split: option.splits code\<^sub>b.splits) 
+text \<open>Evaluation preserves the property of being orderly:\<close>
 
-lemma unflatten_flatten [simp]: "properly_terminated\<^sub>e cd \<Longrightarrow> 
-  unflatten_code (lib @ flatten_code' (length lib) cd @ acc) (length lib + code_list_size cd) = cd"
-proof (induction "length lib" cd arbitrary: lib acc rule: flatten_code'.induct)
-  case (4 cd' cd)
-  let ?pc = "length lib + code_list_size cd'"
-  let ?code' = "lib @ flatten_code' (length lib) cd' @ []"
-  let ?code = "?code' @ flatten_code' ?pc cd @ PushLam\<^sub>b ?pc # acc"
-  have X: "length lib + length (flatten_code' (length lib) cd') = length ?code'" by simp
-  from 4 have "properly_terminated\<^sub>e cd" by simp
-  with 4 X have "unflatten_code (?code' @ flatten_code' (length ?code') cd @
-    PushLam\<^sub>b (length lib + length (flatten_code' (length lib) cd')) # acc)
-      (length ?code' + code_list_size cd) = cd" by blast
-  hence "unflatten_code ?code (length lib + code_list_size cd' + code_list_size cd) = cd" by simp
-  hence X: "unflatten_code ?code (length lib + (code_list_size cd' + code_list_size cd)) = cd" 
-    by (metis add.assoc)
-  from 4 have "properly_terminated\<^sub>e cd'" by simp
-  with 4 have "unflatten_code ?code' (length lib + code_list_size cd') = cd'" by blast
-  moreover have "?pc \<le> length ?code'" by simp
-  ultimately have Z: "unflatten_code ?code ?pc =  cd'" by (metis unflatten_front)
-  with X Z show ?case by simp
-qed simp_all
-
-lemma [simp]: "properly_terminated\<^sub>e cd \<Longrightarrow> unflatten_code (flatten_code cd) (code_list_size cd) = cd"
-proof -
-  assume "properly_terminated\<^sub>e cd"
-  hence "unflatten_code ([] @ flatten_code' (length []) cd @ []) 
-    (length [] + code_list_size cd) = cd" by (metis unflatten_flatten list.size(3))
-  thus ?thesis by (simp add: flatten_code_def)
-qed
-
-lemma orderly_lam [simp]: "lookup cd pc = Some (PushLam\<^sub>b pc') \<Longrightarrow> orderly_code cd n \<Longrightarrow> pc' \<le> pc + n"
-  by (induction cd pc arbitrary: n rule: lookup.induct) fastforce+
-
-lemma [simp]: "lookup cd pc = Some (PushLam\<^sub>b pc') \<Longrightarrow> orderly_code cd 0 \<Longrightarrow> pc' \<le> pc"
-  using orderly_lam by fastforce
-
-theorem completeb [simp]: "cd \<tturnstile> \<Sigma>\<^sub>b \<leadsto>\<^sub>b \<Sigma>\<^sub>b' \<Longrightarrow> orderly_state cd \<Sigma>\<^sub>b \<Longrightarrow> 
-  iter (\<leadsto>\<^sub>e) (unflatten_state cd \<Sigma>\<^sub>b) (unflatten_state cd \<Sigma>\<^sub>b')"
-proof (induction \<Sigma>\<^sub>b \<Sigma>\<^sub>b' rule: eval\<^sub>b.induct)
-  case (ev\<^sub>b_lookup cd pc x env v vs sfs)
-  hence "S\<^sub>e (unflatten_values cd vs) 
-    ((unflatten_values cd env, unflatten_code cd (Suc pc)) # unflatten_stack cd sfs) \<leadsto>\<^sub>e
-      S\<^sub>e (unflatten_closure cd v # unflatten_values cd vs)
-        ((unflatten_values cd env, unflatten_code cd pc) # unflatten_stack cd sfs)" by simp
-  thus ?case by simp
+lemma eval_preserves_orderly [simp]: "\<C>\<^sub>b \<tturnstile> \<Sigma>\<^sub>b \<leadsto>\<^sub>b \<Sigma>\<^sub>b' \<Longrightarrow> orderly_state \<C>\<^sub>b \<Sigma>\<^sub>b \<Longrightarrow> 
+  orderly_state \<C>\<^sub>b \<Sigma>\<^sub>b'"
+proof (induction \<C>\<^sub>b \<Sigma>\<^sub>b \<Sigma>\<^sub>b' rule: eval\<^sub>b.induct)
+  case (ev\<^sub>b_lookup cd pc x env v vs s)
+  thus ?case by (cases pc, cases cd) auto
 next
-  case (ev\<^sub>b_pushcon cd pc k vs env sfs)
-  hence "S\<^sub>e (unflatten_values cd vs) 
-    ((unflatten_values cd env, unflatten_code cd (Suc pc)) # unflatten_stack cd sfs) \<leadsto>\<^sub>e
-      S\<^sub>e (Const\<^sub>e k # unflatten_values cd vs) 
-        ((unflatten_values cd env, unflatten_code cd pc) # unflatten_stack cd sfs)" by simp
-  thus ?case by simp
-next
-  case (ev\<^sub>b_pushlam cd pc pc' vs env sfs)
-  moreover hence X: "pc' \<le> pc" by auto
-  moreover have "iter (\<leadsto>\<^sub>e) (S\<^sub>e (unflatten_values cd vs) ((unflatten_values cd env, 
-    PushLam\<^sub>e (unflatten_code cd pc') # 
-      unflatten_code cd pc) # unflatten_stack cd sfs))
-        (S\<^sub>e (Lam\<^sub>e (unflatten_values cd env) (unflatten_code cd pc') # unflatten_values cd vs) 
-          ((unflatten_values cd env, unflatten_code cd pc) # unflatten_stack cd sfs))" 
-    by (metis ev\<^sub>e_pushlam iter_one)
-  ultimately show ?case by simp
-next
-  case (ev\<^sub>b_apply cd pc v env' pc' vs env sfs)
-  hence "S\<^sub>e (unflatten_closure cd v # Lam\<^sub>e (unflatten_values cd env') (unflatten_code cd pc') # unflatten_values cd vs) 
-      ((unflatten_values cd env, unflatten_code cd (Suc pc)) # unflatten_stack cd sfs) \<leadsto>\<^sub>e
-        S\<^sub>e (unflatten_values cd vs) ((unflatten_closure cd v # unflatten_values cd env', unflatten_code cd pc') # 
-          (unflatten_values cd env, unflatten_code cd pc) # 
-            unflatten_stack cd sfs)" by simp
-  thus ?case by simp
-next
-  case (ev\<^sub>b_return cd pc vs env sfs)
-  moreover have "iter (\<leadsto>\<^sub>e) (S\<^sub>e (unflatten_values cd vs) ((unflatten_values cd env, [Return\<^sub>e]) # unflatten_stack cd sfs))
-    (S\<^sub>e (unflatten_values cd vs) (unflatten_stack cd sfs))" by (metis ev\<^sub>e_return iter_one)
-  ultimately show ?case by simp
-next
-  case (ev\<^sub>b_jump cd pc v env' pc' vs env sfs)
-  have "S\<^sub>e (unflatten_closure cd v # Lam\<^sub>e (unflatten_values cd env') (unflatten_code cd pc') # unflatten_values cd vs) 
-    ((unflatten_values cd env, [Jump\<^sub>e]) # unflatten_stack cd sfs) \<leadsto>\<^sub>e S\<^sub>e (unflatten_values cd vs)
-        ((unflatten_closure cd v # unflatten_values cd env', unflatten_code cd pc') # 
-          unflatten_stack cd sfs)" by (metis ev\<^sub>e_jump)
-  with ev\<^sub>b_jump have "S\<^sub>e (unflatten_closure cd v # 
-    Lam\<^sub>e (unflatten_values cd env') (unflatten_code cd pc') # unflatten_values cd vs)
-      ((unflatten_values cd env, unflatten_code cd (Suc pc)) # unflatten_stack cd sfs) \<leadsto>\<^sub>e
-        S\<^sub>e (unflatten_values cd vs) ((unflatten_closure cd v # unflatten_values cd env', unflatten_code cd pc') # unflatten_stack cd sfs)" by simp
-  hence "iter (\<leadsto>\<^sub>e) (S\<^sub>e (unflatten_closure cd v # 
-    Lam\<^sub>e (unflatten_values cd env') (unflatten_code cd pc') # unflatten_values cd vs)
-      ((unflatten_values cd env, unflatten_code cd (Suc pc)) # unflatten_stack cd sfs))
-        (S\<^sub>e (unflatten_values cd vs) ((unflatten_closure cd v # unflatten_values cd env', unflatten_code cd pc') # unflatten_stack cd sfs))" 
-    by (metis iter_one)
-  thus ?case by simp
-qed
-
-lemma [simp]: "Lam\<^sub>e envt cdt = unflatten_closure cdb vb \<Longrightarrow> 
-  \<exists>envb pc. vb = Lam\<^sub>b envb pc \<and> envt = unflatten_values cdb envb \<and> cdt = unflatten_code cdb pc"
-  by (induction vb) simp_all
-
-lemma unfl_state [dest]: "S\<^sub>e vs sfs = unflatten_state cd \<Sigma>\<^sub>b \<Longrightarrow> \<exists>vsb sfsb. 
-    \<Sigma>\<^sub>b = S\<^sub>b vsb sfsb \<and> vs = unflatten_values cd vsb \<and> sfs = unflatten_stack cd sfsb"
-  by (induction \<Sigma>\<^sub>b) simp_all
-
-lemma [dest]: "Lookup\<^sub>e x # cdt = unflatten_code cdb (Suc pc) \<Longrightarrow> orderly_code cdb 0 \<Longrightarrow> 
-    pc < length cdb \<Longrightarrow> lookup cdb pc = Some (Lookup\<^sub>b x) \<and> cdt = unflatten_code cdb pc"
-  by (simp split: option.splits code\<^sub>b.splits)
-
-lemma [dest]: "PushCon\<^sub>e k # cdt = unflatten_code cdb (Suc pc) \<Longrightarrow> orderly_code cdb 0 \<Longrightarrow> 
-    pc < length cdb \<Longrightarrow> lookup cdb pc = Some (PushCon\<^sub>b k) \<and> cdt = unflatten_code cdb pc"
-  by (simp split: option.splits code\<^sub>b.splits)
-
-lemma [dest]: "PushLam\<^sub>e cdt'' # cdt = unflatten_code cdb (Suc pc) \<Longrightarrow> 
-  orderly_code cdb 0 \<Longrightarrow> pc < length cdb \<Longrightarrow>  
-    \<exists>pc'. lookup cdb pc = Some (PushLam\<^sub>b pc') \<and> cdt = unflatten_code cdb pc \<and> 
-      cdt'' = unflatten_code cdb pc'"
-  by (simp split: option.splits code\<^sub>b.splits)
-
-lemma [dest]: "Apply\<^sub>e # cdt = unflatten_code cdb (Suc pc) \<Longrightarrow> orderly_code cdb 0 \<Longrightarrow> 
-    pc < length cdb \<Longrightarrow> lookup cdb pc = Some Apply\<^sub>b \<and> cdt = unflatten_code cdb pc"
-  by (simp split: option.splits code\<^sub>b.splits)
-
-lemma [dest]: "Return\<^sub>e # cd = unflatten_code cdb (Suc pc) \<Longrightarrow> 
-    orderly_code cdb 0 \<Longrightarrow> pc < length cdb \<Longrightarrow> lookup cdb pc = Some Return\<^sub>b \<and> cd = []"
-  by (simp split: option.splits code\<^sub>b.splits)
-
-lemma [dest]: "Jump\<^sub>e # cd = unflatten_code cdb (Suc pc) \<Longrightarrow> 
-    orderly_code cdb 0 \<Longrightarrow> pc < length cdb \<Longrightarrow> lookup cdb pc = Some Jump\<^sub>b \<and> cd = []"
-  by (simp split: option.splits code\<^sub>b.splits)
-
-lemma uf_to_lookup [dest]: "(envt, Lookup\<^sub>e x # cdt) # sfst = unflatten_stack cdb sfsb \<Longrightarrow> 
-  orderly_code cdb 0 \<Longrightarrow> orderly_stack sfsb (length cdb) \<Longrightarrow> \<exists>envb pc sfsb'. 
-    sfsb = (envb, Suc pc) # sfsb' \<and> envt = unflatten_values cdb envb \<and> lookup cdb pc = Some (Lookup\<^sub>b x) \<and> 
-      cdt = unflatten_code cdb pc \<and> sfst = unflatten_stack cdb sfsb'"
-proof (induction sfsb "length cdb" rule: orderly_stack.induct)
-  case (3 envb pc sfsb')
-  hence "Lookup\<^sub>e x # cdt = unflatten_code cdb (Suc pc) \<and> orderly_code cdb 0 \<and> pc < length cdb" by simp
-  hence "lookup cdb pc = Some (Lookup\<^sub>b x) \<and> cdt = unflatten_code cdb pc" by blast
-  with 3 show ?case by simp
-qed simp_all
-
-lemma uf_to_pushcon [dest]: "(envt, PushCon\<^sub>e k # cdt) # sfst = unflatten_stack cdb sfsb \<Longrightarrow> 
-  orderly_code cdb 0 \<Longrightarrow> orderly_stack sfsb (length cdb) \<Longrightarrow> 
-    \<exists>envb pc sfsb'. sfsb = (envb, Suc pc) # sfsb' \<and> envt = unflatten_values cdb envb \<and> 
-      lookup cdb pc = Some (PushCon\<^sub>b k) \<and> cdt = unflatten_code cdb pc \<and> sfst = unflatten_stack cdb sfsb'"
-proof (induction sfsb "length cdb" rule: orderly_stack.induct)
-  case (3 envb pc sfsb')
-  hence "PushCon\<^sub>e k # cdt = unflatten_code cdb (Suc pc) \<and> orderly_code cdb 0 \<and> pc < length cdb" by simp
-  hence "lookup cdb pc = Some (PushCon\<^sub>b k) \<and> cdt = unflatten_code cdb pc" by blast
-  with 3 show ?case by simp
-qed simp_all
-
-lemma uf_to_pushlam [dest]: "(envt, PushLam\<^sub>e cdt' # cdt) # sfst = unflatten_stack cdb sfsb \<Longrightarrow> 
-  orderly_code cdb 0 \<Longrightarrow> orderly_stack sfsb (length cdb) \<Longrightarrow> \<exists>envb pc sfsb' pc'. 
-    sfsb = (envb, Suc pc) # sfsb' \<and> envt = unflatten_values cdb envb \<and> lookup cdb pc = Some (PushLam\<^sub>b pc') \<and> 
-      cdt = unflatten_code cdb pc \<and> cdt' = unflatten_code cdb pc' \<and> sfst = unflatten_stack cdb sfsb'"
-proof (induction sfsb "length cdb" rule: orderly_stack.induct)
-  case (3 envb pc sfsb')
-  hence "PushLam\<^sub>e cdt' # cdt = unflatten_code cdb (Suc pc) \<and> orderly_code cdb 0 \<and> pc < length cdb" 
-    by simp
-  then obtain pc' where "lookup cdb pc = Some (PushLam\<^sub>b pc') \<and> cdt = unflatten_code cdb pc \<and> 
-    cdt' = unflatten_code cdb pc'" by blast
-  with 3 show ?case by simp
-qed simp_all
-
-lemma uf_to_apply [dest]: "(envt, Apply\<^sub>e # cdt) # sfst = unflatten_stack cdb sfsb \<Longrightarrow> orderly_code cdb 0 \<Longrightarrow> 
-  orderly_stack sfsb (length cdb) \<Longrightarrow> \<exists>envb pc sfsb'. sfsb = (envb, Suc pc) # sfsb' \<and> 
-    envt = unflatten_values cdb envb \<and> lookup cdb pc = Some Apply\<^sub>b \<and> cdt = unflatten_code cdb pc \<and> 
-      sfst = unflatten_stack cdb sfsb'"
-proof (induction sfsb "length cdb" rule: orderly_stack.induct)
-  case (3 envb pc sfsb')
-  hence "Apply\<^sub>e # cdt = unflatten_code cdb (Suc pc) \<and> orderly_code cdb 0 \<and> pc < length cdb" by simp
-  hence "lookup cdb pc = Some Apply\<^sub>b \<and> cdt = unflatten_code cdb pc" by blast
-  with 3 show ?case by simp
-qed simp_all
-
-lemma uf_to_return [dest]: "(envt, Return\<^sub>e # cd) # sfst = unflatten_stack cdb sfsb \<Longrightarrow> orderly_code cdb 0 \<Longrightarrow> 
-  orderly_stack sfsb (length cdb) \<Longrightarrow> \<exists>envb pc sfsb'. sfsb = (envb, Suc pc) # sfsb' \<and> 
-    envt = unflatten_values cdb envb \<and> lookup cdb pc = Some Return\<^sub>b \<and> sfst = unflatten_stack cdb sfsb' \<and> cd = []"
-proof (induction sfsb "length cdb" rule: orderly_stack.induct)
-  case (3 envb pc sfsb')
-  hence "Return\<^sub>e # cd = unflatten_code cdb (Suc pc) \<and> 
-    orderly_code cdb 0 \<and> pc < length cdb" by simp
-  hence "lookup cdb pc = Some Return\<^sub>b \<and> cd = []" by blast
-  with 3 show ?case by simp
-qed simp_all
-
-lemma uf_to_jump [dest]: "(envt, Jump\<^sub>e # cd) # sfst = unflatten_stack cdb sfsb \<Longrightarrow> orderly_code cdb 0 \<Longrightarrow> 
-  orderly_stack sfsb (length cdb) \<Longrightarrow> \<exists>envb pc sfsb'. sfsb = (envb, Suc pc) # sfsb' \<and> 
-    envt = unflatten_values cdb envb \<and> lookup cdb pc = Some Jump\<^sub>b \<and> sfst = unflatten_stack cdb sfsb'"
-proof (induction sfsb "length cdb" rule: orderly_stack.induct)
-  case (3 envb pc sfsb')
-  hence "Jump\<^sub>e # cd = unflatten_code cdb (Suc pc) \<and> 
-    orderly_code cdb 0 \<and> pc < length cdb" by simp
-  hence "lookup cdb pc = Some Jump\<^sub>b \<and> cd = []" by blast
-  with 3 show ?case by simp
-qed simp_all
-
-theorem correctb [simp]: "unflatten_state cd\<^sub>b \<Sigma>\<^sub>b \<leadsto>\<^sub>e \<Sigma>\<^sub>t' \<Longrightarrow> orderly_state cd\<^sub>b \<Sigma>\<^sub>b \<Longrightarrow>
-  \<exists>\<Sigma>\<^sub>b'. iter (\<tturnstile> cd\<^sub>b \<leadsto>\<^sub>b) \<Sigma>\<^sub>b \<Sigma>\<^sub>b' \<and> unflatten_state cd\<^sub>b \<Sigma>\<^sub>b' = \<Sigma>\<^sub>t'"
-proof (induction "unflatten_state cd\<^sub>b \<Sigma>\<^sub>b" \<Sigma>\<^sub>t' rule: eval\<^sub>e.induct)
-  case (ev\<^sub>e_lookup env x v vs cd sfs)
-  then obtain vsb sfsb where B: "\<Sigma>\<^sub>b = S\<^sub>b vsb sfsb \<and> vs = unflatten_values cd\<^sub>b vsb \<and> 
-    (env, Lookup\<^sub>e x # cd) # sfs = unflatten_stack cd\<^sub>b sfsb" by fastforce
-  with ev\<^sub>e_lookup have "orderly_code cd\<^sub>b 0 \<and> orderly_stack sfsb (length cd\<^sub>b)" by simp
-  with B obtain envb pc sfsb' where S: "sfsb = (envb, Suc pc) # sfsb' \<and> 
-    env = unflatten_values cd\<^sub>b envb \<and> lookup cd\<^sub>b pc = Some (Lookup\<^sub>b x) \<and> cd = unflatten_code cd\<^sub>b pc \<and> 
-      sfs = unflatten_stack cd\<^sub>b sfsb'" by (metis uf_to_lookup)
-  with ev\<^sub>e_lookup obtain v' where V: "lookup envb x = Some v' \<and> unflatten_closure cd\<^sub>b v' = v"
-    by fastforce
-  with S have "cd\<^sub>b \<tturnstile> S\<^sub>b vsb ((envb, Suc pc) # sfsb') \<leadsto>\<^sub>b S\<^sub>b (v' # vsb) ((envb, pc) # sfsb')"
-    by simp
-  hence "iter (\<tturnstile> cd\<^sub>b \<leadsto>\<^sub>b) (S\<^sub>b vsb ((envb, Suc pc) # sfsb')) (S\<^sub>b (v' # vsb) ((envb, pc) # sfsb'))" 
-    by simp
-  with B S V show ?case by fastforce
-next
-  case (ev\<^sub>e_pushcon vs env k cd sfs)
-  then obtain vsb sfsb where B: "\<Sigma>\<^sub>b = S\<^sub>b vsb sfsb \<and> vs = unflatten_values cd\<^sub>b vsb \<and> 
-    (env, PushCon\<^sub>e k # cd) # sfs = unflatten_stack cd\<^sub>b sfsb" by fastforce
-  with ev\<^sub>e_pushcon have "orderly_code cd\<^sub>b 0 \<and> orderly_stack sfsb (length cd\<^sub>b)" by simp
-  with B obtain envb pc sfsb' where S: "sfsb = (envb, Suc pc) # sfsb' \<and> 
-    env = unflatten_values cd\<^sub>b envb \<and> lookup cd\<^sub>b pc = Some (PushCon\<^sub>b k) \<and> cd = unflatten_code cd\<^sub>b pc \<and> 
-      sfs = unflatten_stack cd\<^sub>b sfsb'" by (metis uf_to_pushcon)
-  with S have "cd\<^sub>b \<tturnstile> S\<^sub>b vsb ((envb, Suc pc) # sfsb') \<leadsto>\<^sub>b S\<^sub>b (Const\<^sub>b k # vsb) ((envb, pc) # sfsb')"
-    by simp
-  hence "iter (\<tturnstile> cd\<^sub>b \<leadsto>\<^sub>b) (S\<^sub>b vsb ((envb, Suc pc) # sfsb')) 
-    (S\<^sub>b (Const\<^sub>b k # vsb) ((envb, pc) # sfsb'))" by simp
-  with B S show ?case by fastforce
-next
-  case (ev\<^sub>e_pushlam vs env cd' cd sfs)
-  then obtain vsb sfsb where B: "\<Sigma>\<^sub>b = S\<^sub>b vsb sfsb \<and> vs = unflatten_values cd\<^sub>b vsb \<and> 
-    (env, PushLam\<^sub>e cd' # cd) # sfs = unflatten_stack cd\<^sub>b sfsb" by fastforce
-  with ev\<^sub>e_pushlam have "orderly_code cd\<^sub>b 0 \<and> orderly_stack sfsb (length cd\<^sub>b)" by simp
-  with B obtain envb pc sfsb' pc' where S: "sfsb = (envb, Suc pc) # sfsb' \<and> 
-    env = unflatten_values cd\<^sub>b envb \<and> lookup cd\<^sub>b pc = Some (PushLam\<^sub>b pc') \<and> cd = unflatten_code cd\<^sub>b pc \<and> 
-      sfs = unflatten_stack cd\<^sub>b sfsb' \<and> cd' = unflatten_code cd\<^sub>b pc'" by (metis uf_to_pushlam)
-  with S have "cd\<^sub>b \<tturnstile> S\<^sub>b vsb ((envb, Suc pc) # sfsb') \<leadsto>\<^sub>b 
-    S\<^sub>b (Lam\<^sub>b envb pc' # vsb) ((envb, pc) # sfsb')" by simp
-  hence "iter (\<tturnstile> cd\<^sub>b \<leadsto>\<^sub>b) (S\<^sub>b vsb ((envb, Suc pc) # sfsb')) 
-    (S\<^sub>b (Lam\<^sub>b envb pc' # vsb) ((envb, pc) # sfsb'))" by simp
-  with B S show ?case by fastforce
-next
-  case (ev\<^sub>e_apply v env' cd' vs env cd sfs)
-  then obtain vsb sfsb where B: "\<Sigma>\<^sub>b = S\<^sub>b vsb sfsb \<and> 
-    v # Lam\<^sub>e env' cd' # vs = unflatten_values cd\<^sub>b vsb \<and> (env, Apply\<^sub>e # cd) # sfs = unflatten_stack cd\<^sub>b sfsb" 
-      by fastforce
-  with ev\<^sub>e_apply have "orderly_code cd\<^sub>b 0 \<and> orderly_stack sfsb (length cd\<^sub>b)" by simp
-  with B obtain envb pc sfsb' where S: "sfsb = (envb, Suc pc) # sfsb' \<and> 
-    env = unflatten_values cd\<^sub>b envb \<and> lookup cd\<^sub>b pc = Some Apply\<^sub>b \<and> cd = unflatten_code cd\<^sub>b pc \<and> 
-      sfs = unflatten_stack cd\<^sub>b sfsb'" by (metis uf_to_apply)
-  from B obtain vb envb' pc' vsb' where V: "vsb = vb # Lam\<^sub>b envb' pc' # vsb' \<and> 
-    v = unflatten_closure cd\<^sub>b vb \<and> env' = unflatten_values cd\<^sub>b envb' \<and> cd' = unflatten_code cd\<^sub>b pc' \<and>
-      vs = unflatten_values cd\<^sub>b vsb'" by fastforce
-  from S have "cd\<^sub>b \<tturnstile> S\<^sub>b (vb # Lam\<^sub>b envb' pc' # vsb') ((envb, Suc pc) # sfsb') \<leadsto>\<^sub>b
-    S\<^sub>b vsb' ((vb # envb', pc') # (envb, pc) # sfsb')" by simp
-  hence "iter (\<tturnstile> cd\<^sub>b \<leadsto>\<^sub>b) (S\<^sub>b (vb # Lam\<^sub>b envb' pc' # vsb') ((envb, Suc pc) # sfsb')) 
-    (S\<^sub>b vsb' ((vb # envb', pc') # (envb, pc) # sfsb'))" by simp
-  with B S V show ?case by auto                                              
-next
-  case (ev\<^sub>e_return vs env cd sfs)
-  then obtain vsb sfsb where B: "\<Sigma>\<^sub>b = S\<^sub>b vsb sfsb \<and> vs = unflatten_values cd\<^sub>b vsb \<and> 
-    (env, Return\<^sub>e # cd) # sfs = unflatten_stack cd\<^sub>b sfsb" by fastforce
-  with ev\<^sub>e_return have "orderly_code cd\<^sub>b 0 \<and> orderly_stack sfsb (length cd\<^sub>b)" by simp
-  with B obtain envb pc sfsb' where S: "sfsb = (envb, Suc pc) # sfsb' \<and> 
-    env = unflatten_values cd\<^sub>b envb \<and> lookup cd\<^sub>b pc = Some Return\<^sub>b \<and> sfs = unflatten_stack cd\<^sub>b sfsb'" 
-      by (metis uf_to_return)
-  with S have "cd\<^sub>b \<tturnstile> S\<^sub>b vsb ((envb, Suc pc) # sfsb') \<leadsto>\<^sub>b S\<^sub>b vsb sfsb'" by simp
-  hence "iter (\<tturnstile> cd\<^sub>b \<leadsto>\<^sub>b) (S\<^sub>b vsb ((envb, Suc pc) # sfsb')) (S\<^sub>b vsb sfsb')" by simp
-  with B S show ?case by fastforce
-next
-  case (ev\<^sub>e_jump v env' cd' vs env cd sfs)
-  then obtain vsb sfsb where B: "\<Sigma>\<^sub>b = S\<^sub>b vsb sfsb \<and> 
-    v # Lam\<^sub>e env' cd' # vs = unflatten_values cd\<^sub>b vsb \<and> 
-      (env, Jump\<^sub>e # cd) # sfs = unflatten_stack cd\<^sub>b sfsb" by fastforce
-  with ev\<^sub>e_jump have "orderly_code cd\<^sub>b 0 \<and> orderly_stack sfsb (length cd\<^sub>b)" by simp
-  with B obtain envb pc sfsb' where S: "sfsb = (envb, Suc pc) # sfsb' \<and> 
-    env = unflatten_values cd\<^sub>b envb \<and> lookup cd\<^sub>b pc = Some Jump\<^sub>b \<and> sfs = unflatten_stack cd\<^sub>b sfsb'" 
-      by (metis uf_to_jump)
-  from B obtain vb envb' pc' vsb' where V: "vsb = vb # Lam\<^sub>b envb' pc' # vsb' \<and> 
-    v = unflatten_closure cd\<^sub>b vb \<and> env' = unflatten_values cd\<^sub>b envb' \<and> cd' = unflatten_code cd\<^sub>b pc' \<and>
-      vs = unflatten_values cd\<^sub>b vsb'" by fastforce
-  from S have "cd\<^sub>b \<tturnstile> S\<^sub>b (vb # Lam\<^sub>b envb' pc' # vsb') ((envb, Suc pc) # sfsb') \<leadsto>\<^sub>b
-    S\<^sub>b vsb' ((vb # envb', pc') # sfsb')" by simp
-  hence "iter (\<tturnstile> cd\<^sub>b \<leadsto>\<^sub>b) (S\<^sub>b (vb # Lam\<^sub>b envb' pc' # vsb') ((envb, Suc pc) # sfsb')) 
-    (S\<^sub>b vsb' ((vb # envb', pc') # sfsb'))" by simp
-  with B S V show ?case by auto                                              
-qed
-
-lemma [simp]: "cd\<^sub>b \<tturnstile> \<Sigma>\<^sub>b \<leadsto>\<^sub>b \<Sigma>\<^sub>b' \<Longrightarrow> orderly_state cd\<^sub>b \<Sigma>\<^sub>b \<Longrightarrow> orderly_state cd\<^sub>b \<Sigma>\<^sub>b'"
-proof (induction cd\<^sub>b \<Sigma>\<^sub>b \<Sigma>\<^sub>b' rule: eval\<^sub>b.induct)
-  case (ev\<^sub>b_lookup cd pc x env v vs sfs)
+  case (ev\<^sub>b_pushcon cd pc k vs env s)
   thus ?case by (cases pc, cases cd) simp_all
 next
-  case (ev\<^sub>b_pushcon cd pc k vs env sfs)
-  thus ?case by (cases pc, cases cd) simp_all
-next
-  case (ev\<^sub>b_pushlam cd pc pc' vs env sfs)
+  case (ev\<^sub>b_pushlam cd pc pc' vs env s)
   thus ?case 
   proof (cases pc)
     case 0
     with ev\<^sub>b_pushlam show ?thesis by (cases cd) simp_all
   qed simp_all
 next
-  case (ev\<^sub>b_apply cd pc v env' pc' vs env sfs)
+  case (ev\<^sub>b_apply cd pc v env' pc' vs env s)
   thus ?case by (cases pc', simp, cases pc, cases cd) simp_all
 next
-  case (ev\<^sub>b_jump cd pc v env' pc' vs env sfs)
+  case (ev\<^sub>b_jump cd pc v env' pc' vs env s)
   thus ?case by (cases pc') simp_all
 qed simp_all
 
-lemma [simp]: "iter (\<tturnstile> cd\<^sub>b \<leadsto>\<^sub>b) \<Sigma>\<^sub>b \<Sigma>\<^sub>b' \<Longrightarrow> orderly_state cd\<^sub>b \<Sigma>\<^sub>b \<Longrightarrow> orderly_state cd\<^sub>b \<Sigma>\<^sub>b'"
+lemma iter_eval_preserves_orderly [simp]: "iter (\<tturnstile> \<C>\<^sub>b \<leadsto>\<^sub>b) \<Sigma>\<^sub>b \<Sigma>\<^sub>b' \<Longrightarrow> orderly_state \<C>\<^sub>b \<Sigma>\<^sub>b \<Longrightarrow> 
+    orderly_state \<C>\<^sub>b \<Sigma>\<^sub>b'"
   by (induction \<Sigma>\<^sub>b \<Sigma>\<^sub>b' rule: iter.induct) simp_all
 
-lemma [simp]: "iter (\<leadsto>\<^sub>e) (unflatten_state cd\<^sub>b \<Sigma>\<^sub>b) \<Sigma>\<^sub>t' \<Longrightarrow> orderly_state cd\<^sub>b \<Sigma>\<^sub>b \<Longrightarrow>
-  \<exists>\<Sigma>\<^sub>b'. iter (\<tturnstile> cd\<^sub>b \<leadsto>\<^sub>b) \<Sigma>\<^sub>b \<Sigma>\<^sub>b' \<and> unflatten_state cd\<^sub>b \<Sigma>\<^sub>b' = \<Sigma>\<^sub>t'"
-proof (induction "unflatten_state cd\<^sub>b \<Sigma>\<^sub>b" \<Sigma>\<^sub>t' arbitrary: \<Sigma>\<^sub>b rule: iter.induct)
-  case (iter_step \<Sigma>\<^sub>t' \<Sigma>\<^sub>t'')
-  moreover then obtain \<Sigma>\<^sub>b' where S: "iter (\<tturnstile> cd\<^sub>b \<leadsto>\<^sub>b) \<Sigma>\<^sub>b \<Sigma>\<^sub>b' \<and> unflatten_state cd\<^sub>b \<Sigma>\<^sub>b' = \<Sigma>\<^sub>t'" 
+text \<open>Because we use an unflattening function rather than a flattening one, completeness is 
+straightforward:\<close>
+
+theorem complete\<^sub>b [simp]: "\<C> \<tturnstile> \<Sigma>\<^sub>b \<leadsto>\<^sub>b \<Sigma>\<^sub>b' \<Longrightarrow> orderly_state \<C> \<Sigma>\<^sub>b \<Longrightarrow> 
+  iter (\<leadsto>\<^sub>e) (unflatten_state \<C> \<Sigma>\<^sub>b) (unflatten_state \<C> \<Sigma>\<^sub>b')"
+proof (induction \<Sigma>\<^sub>b \<Sigma>\<^sub>b' rule: eval\<^sub>b.induct)
+  case (ev\<^sub>b_lookup \<C> p x \<Delta> v \<V> s)
+  hence "S\<^sub>e (unflatten_values \<C> \<V>) ((unflatten_values \<C> \<Delta>, unflatten_code \<C> (Suc p)) # 
+    unflatten_stack \<C> s) \<leadsto>\<^sub>e
+    S\<^sub>e (unflatten_closure \<C> v # unflatten_values \<C> \<V>) ((unflatten_values \<C> \<Delta>, unflatten_code \<C> p) # 
+    unflatten_stack \<C> s)" by simp
+  thus ?case by simp
+next
+  case (ev\<^sub>b_pushcon \<C> p k \<V> \<Delta> s)
+  hence "S\<^sub>e (unflatten_values \<C> \<V>) ((unflatten_values \<C> \<Delta>, unflatten_code \<C> (Suc p)) # 
+    unflatten_stack \<C> s) \<leadsto>\<^sub>e
+    S\<^sub>e (Const\<^sub>e k # unflatten_values \<C> \<V>) ((unflatten_values \<C> \<Delta>, unflatten_code \<C> p) # 
+    unflatten_stack \<C> s)" by simp
+  thus ?case by simp
+next
+  case (ev\<^sub>b_pushlam \<C> p p' \<V> \<Delta> s)
+  moreover hence X: "p' \<le> p" by auto
+  moreover have "iter (\<leadsto>\<^sub>e) (S\<^sub>e (unflatten_values \<C> \<V>) ((unflatten_values \<C> \<Delta>, 
+    PushLam\<^sub>e (unflatten_code \<C> p') # unflatten_code \<C> p) # unflatten_stack \<C> s))
+    (S\<^sub>e (Lam\<^sub>e (unflatten_values \<C> \<Delta>) (unflatten_code \<C> p') # unflatten_values \<C> \<V>) 
+    ((unflatten_values \<C> \<Delta>, unflatten_code \<C> p) # unflatten_stack \<C> s))" 
+      by (metis ev\<^sub>e_pushlam iter_one)
+  ultimately show ?case by simp
+next
+  case (ev\<^sub>b_apply \<C> p v \<Delta>' p' \<V> \<Delta> s)
+  hence "S\<^sub>e (unflatten_closure \<C> v # Lam\<^sub>e (unflatten_values \<C> \<Delta>') (unflatten_code \<C> p') # 
+    unflatten_values \<C> \<V>) 
+    ((unflatten_values \<C> \<Delta>, unflatten_code \<C> (Suc p)) # unflatten_stack \<C> s) \<leadsto>\<^sub>e
+    S\<^sub>e (unflatten_values \<C> \<V>) ((unflatten_closure \<C> v # unflatten_values \<C> \<Delta>', 
+    unflatten_code \<C> p') # (unflatten_values \<C> \<Delta>, unflatten_code \<C> p) # unflatten_stack \<C> s)" 
+      by simp
+  thus ?case by simp
+next
+  case (ev\<^sub>b_return \<C> p \<V> \<Delta> s)
+  moreover have "iter (\<leadsto>\<^sub>e) (S\<^sub>e (unflatten_values \<C> \<V>) ((unflatten_values \<C> \<Delta>, [Return\<^sub>e]) # 
+    unflatten_stack \<C> s))
+    (S\<^sub>e (unflatten_values \<C> \<V>) (unflatten_stack \<C> s))" by (metis ev\<^sub>e_return iter_one)
+  ultimately show ?case by simp
+next
+  case (ev\<^sub>b_jump \<C> p v \<Delta>' p' \<V> \<Delta> s)
+  have "S\<^sub>e (unflatten_closure \<C> v # Lam\<^sub>e (unflatten_values \<C> \<Delta>') (unflatten_code \<C> p') # 
+    unflatten_values \<C> \<V>) ((unflatten_values \<C> \<Delta>, [Jump\<^sub>e]) # unflatten_stack \<C> s) \<leadsto>\<^sub>e 
+    S\<^sub>e (unflatten_values \<C> \<V>) ((unflatten_closure \<C> v # unflatten_values \<C> \<Delta>', 
+    unflatten_code \<C> p') # unflatten_stack \<C> s)" by (metis ev\<^sub>e_jump)
+  with ev\<^sub>b_jump have "S\<^sub>e (unflatten_closure \<C> v # 
+    Lam\<^sub>e (unflatten_values \<C> \<Delta>') (unflatten_code \<C> p') # unflatten_values \<C> \<V>)
+    ((unflatten_values \<C> \<Delta>, unflatten_code \<C> (Suc p)) # unflatten_stack \<C> s) \<leadsto>\<^sub>e
+    S\<^sub>e (unflatten_values \<C> \<V>) ((unflatten_closure \<C> v # unflatten_values \<C> \<Delta>', 
+    unflatten_code \<C> p') # unflatten_stack \<C> s)" by simp
+  hence "iter (\<leadsto>\<^sub>e) (S\<^sub>e (unflatten_closure \<C> v # 
+    Lam\<^sub>e (unflatten_values \<C> \<Delta>') (unflatten_code \<C> p') # unflatten_values \<C> \<V>)
+    ((unflatten_values \<C> \<Delta>, unflatten_code \<C> (Suc p)) # unflatten_stack \<C> s))
+    (S\<^sub>e (unflatten_values \<C> \<V>) ((unflatten_closure \<C> v # unflatten_values \<C> \<Delta>', 
+    unflatten_code \<C> p') # unflatten_stack \<C> s))" 
+      by (metis iter_one)
+  thus ?case by simp
+qed
+
+text \<open>But it means correctness needs the usual supply of reconstruction lemmas.\<close>
+
+lemma unflatten_to_lookup [dest]: "Lookup\<^sub>e x # \<C>\<^sub>e = unflatten_code \<C>\<^sub>b (Suc p) \<Longrightarrow> 
+  orderly_code \<C>\<^sub>b 0 \<Longrightarrow> p < length \<C>\<^sub>b \<Longrightarrow> 
+    lookup \<C>\<^sub>b p = Some (Lookup\<^sub>b x) \<and> \<C>\<^sub>e = unflatten_code \<C>\<^sub>b p"
+  by (simp split: option.splits code\<^sub>b.splits)
+
+lemma unflatten_to_pushcon [dest]: "PushCon\<^sub>e n # \<C>\<^sub>e = unflatten_code \<C>\<^sub>b (Suc p) \<Longrightarrow> 
+  orderly_code \<C>\<^sub>b 0 \<Longrightarrow> p < length \<C>\<^sub>b \<Longrightarrow> 
+    lookup \<C>\<^sub>b p = Some (PushCon\<^sub>b n) \<and> \<C>\<^sub>e = unflatten_code \<C>\<^sub>b p"
+  by (simp split: option.splits code\<^sub>b.splits)
+
+lemma unflatten_to_pushlam [dest]: "PushLam\<^sub>e \<C>\<^sub>e' # \<C>\<^sub>e = unflatten_code \<C>\<^sub>b (Suc p) \<Longrightarrow> 
+  orderly_code \<C>\<^sub>b 0 \<Longrightarrow> p < length \<C>\<^sub>b \<Longrightarrow>  
+    \<exists>p'. lookup \<C>\<^sub>b p = Some (PushLam\<^sub>b p') \<and> \<C>\<^sub>e = unflatten_code \<C>\<^sub>b p \<and> \<C>\<^sub>e' = unflatten_code \<C>\<^sub>b p'"
+  by (simp split: option.splits code\<^sub>b.splits)
+
+lemma unflatten_to_apply [dest]: "Apply\<^sub>e # \<C>\<^sub>e = unflatten_code \<C>\<^sub>b (Suc p) \<Longrightarrow> orderly_code \<C>\<^sub>b 0 \<Longrightarrow> 
+    p < length \<C>\<^sub>b \<Longrightarrow> lookup \<C>\<^sub>b p = Some Apply\<^sub>b \<and> \<C>\<^sub>e = unflatten_code \<C>\<^sub>b p"
+  by (simp split: option.splits code\<^sub>b.splits)
+
+lemma unflatten_to_return [dest]: "Return\<^sub>e # \<C>\<^sub>e = unflatten_code \<C>\<^sub>b (Suc p) \<Longrightarrow> 
+    orderly_code \<C>\<^sub>b 0 \<Longrightarrow> p < length \<C>\<^sub>b \<Longrightarrow> lookup \<C>\<^sub>b p = Some Return\<^sub>b \<and> \<C>\<^sub>e = []"
+  by (simp split: option.splits code\<^sub>b.splits)
+
+lemma unflatten_to_jump [dest]: "Jump\<^sub>e # \<C>\<^sub>e = unflatten_code \<C>\<^sub>b (Suc p) \<Longrightarrow> 
+    orderly_code \<C>\<^sub>b 0 \<Longrightarrow> p < length \<C>\<^sub>b \<Longrightarrow> lookup \<C>\<^sub>b p = Some Jump\<^sub>b \<and> \<C>\<^sub>e = []"
+  by (simp split: option.splits code\<^sub>b.splits)
+
+lemma unflatten_stack_to_lookup [dest]: "(\<Delta>\<^sub>e, Lookup\<^sub>e x # \<C>\<^sub>e) # s\<^sub>e = unflatten_stack \<C>\<^sub>b s\<^sub>b \<Longrightarrow> 
+  orderly_code \<C>\<^sub>b 0 \<Longrightarrow> orderly_stack s\<^sub>b (length \<C>\<^sub>b) \<Longrightarrow> \<exists>\<Delta>\<^sub>b p s\<^sub>b'. 
+    s\<^sub>b = (\<Delta>\<^sub>b, Suc p) # s\<^sub>b' \<and> \<Delta>\<^sub>e = unflatten_values \<C>\<^sub>b \<Delta>\<^sub>b \<and> lookup \<C>\<^sub>b p = Some (Lookup\<^sub>b x) \<and> 
+      \<C>\<^sub>e = unflatten_code \<C>\<^sub>b p \<and> s\<^sub>e = unflatten_stack \<C>\<^sub>b s\<^sub>b'"
+proof (induction s\<^sub>b "length \<C>\<^sub>b" rule: orderly_stack.induct)
+  case (3 \<Delta>\<^sub>b p s\<^sub>b')
+  hence "Lookup\<^sub>e x # \<C>\<^sub>e = unflatten_code \<C>\<^sub>b (Suc p) \<and> orderly_code \<C>\<^sub>b 0 \<and> p < length \<C>\<^sub>b" by simp
+  hence "lookup \<C>\<^sub>b p = Some (Lookup\<^sub>b x) \<and> \<C>\<^sub>e = unflatten_code \<C>\<^sub>b p" by blast
+  with 3 show ?case by simp
+qed simp_all
+
+lemma unflatten_stack_to_pushcon [dest]: "(\<Delta>\<^sub>e, PushCon\<^sub>e n # \<C>\<^sub>e) # s\<^sub>e = unflatten_stack \<C>\<^sub>b s\<^sub>b \<Longrightarrow> 
+  orderly_code \<C>\<^sub>b 0 \<Longrightarrow> orderly_stack s\<^sub>b (length \<C>\<^sub>b) \<Longrightarrow> 
+    \<exists>\<Delta>\<^sub>b p s\<^sub>b'. s\<^sub>b = (\<Delta>\<^sub>b, Suc p) # s\<^sub>b' \<and> \<Delta>\<^sub>e = unflatten_values \<C>\<^sub>b \<Delta>\<^sub>b \<and> 
+      lookup \<C>\<^sub>b p = Some (PushCon\<^sub>b n) \<and> \<C>\<^sub>e = unflatten_code \<C>\<^sub>b p \<and> s\<^sub>e = unflatten_stack \<C>\<^sub>b s\<^sub>b'"
+proof (induction s\<^sub>b "length \<C>\<^sub>b" rule: orderly_stack.induct)
+  case (3 \<Delta>\<^sub>b p s\<^sub>b')
+  hence "PushCon\<^sub>e n # \<C>\<^sub>e = unflatten_code \<C>\<^sub>b (Suc p) \<and> orderly_code \<C>\<^sub>b 0 \<and> p < length \<C>\<^sub>b" by simp
+  hence "lookup \<C>\<^sub>b p = Some (PushCon\<^sub>b n) \<and> \<C>\<^sub>e = unflatten_code \<C>\<^sub>b p" by blast
+  with 3 show ?case by simp
+qed simp_all
+
+lemma unflatten_stack_to_pushlam [dest]: "(\<Delta>\<^sub>e, PushLam\<^sub>e \<C>\<^sub>e' # \<C>\<^sub>e) # s\<^sub>e = unflatten_stack \<C>\<^sub>b s\<^sub>b \<Longrightarrow> 
+  orderly_code \<C>\<^sub>b 0 \<Longrightarrow> orderly_stack s\<^sub>b (length \<C>\<^sub>b) \<Longrightarrow> \<exists>\<Delta>\<^sub>b p s\<^sub>b' p'. 
+    s\<^sub>b = (\<Delta>\<^sub>b, Suc p) # s\<^sub>b' \<and> \<Delta>\<^sub>e = unflatten_values \<C>\<^sub>b \<Delta>\<^sub>b \<and> lookup \<C>\<^sub>b p = Some (PushLam\<^sub>b p') \<and> 
+      \<C>\<^sub>e = unflatten_code \<C>\<^sub>b p \<and> \<C>\<^sub>e' = unflatten_code \<C>\<^sub>b p' \<and> s\<^sub>e = unflatten_stack \<C>\<^sub>b s\<^sub>b'"
+proof (induction s\<^sub>b "length \<C>\<^sub>b" rule: orderly_stack.induct)
+  case (3 \<Delta>\<^sub>b p s\<^sub>b')
+  hence "PushLam\<^sub>e \<C>\<^sub>e' # \<C>\<^sub>e = unflatten_code \<C>\<^sub>b (Suc p) \<and> orderly_code \<C>\<^sub>b 0 \<and> p < length \<C>\<^sub>b" 
+    by simp
+  then obtain p' where "lookup \<C>\<^sub>b p = Some (PushLam\<^sub>b p') \<and> \<C>\<^sub>e = unflatten_code \<C>\<^sub>b p \<and> 
+    \<C>\<^sub>e' = unflatten_code \<C>\<^sub>b p'" by blast
+  with 3 show ?case by simp
+qed simp_all
+
+lemma unflatten_stack_to_apply [dest]: "(\<Delta>\<^sub>e, Apply\<^sub>e # \<C>\<^sub>e) # s\<^sub>e = unflatten_stack \<C>\<^sub>b s\<^sub>b \<Longrightarrow> 
+  orderly_code \<C>\<^sub>b 0 \<Longrightarrow> orderly_stack s\<^sub>b (length \<C>\<^sub>b) \<Longrightarrow> \<exists>\<Delta>\<^sub>b p s\<^sub>b'. s\<^sub>b = (\<Delta>\<^sub>b, Suc p) # s\<^sub>b' \<and> 
+    \<Delta>\<^sub>e = unflatten_values \<C>\<^sub>b \<Delta>\<^sub>b \<and> lookup \<C>\<^sub>b p = Some Apply\<^sub>b \<and> \<C>\<^sub>e = unflatten_code \<C>\<^sub>b p \<and> 
+      s\<^sub>e = unflatten_stack \<C>\<^sub>b s\<^sub>b'"
+proof (induction s\<^sub>b "length \<C>\<^sub>b" rule: orderly_stack.induct)
+  case (3 \<Delta>\<^sub>b p s\<^sub>b')
+  hence "Apply\<^sub>e # \<C>\<^sub>e = unflatten_code \<C>\<^sub>b (Suc p) \<and> orderly_code \<C>\<^sub>b 0 \<and> p < length \<C>\<^sub>b" by simp
+  hence "lookup \<C>\<^sub>b p = Some Apply\<^sub>b \<and> \<C>\<^sub>e = unflatten_code \<C>\<^sub>b p" by blast
+  with 3 show ?case by simp
+qed simp_all
+
+lemma unflatten_stack_to_return [dest]: "(\<Delta>\<^sub>e, Return\<^sub>e # \<C>\<^sub>e) # s\<^sub>e = unflatten_stack \<C>\<^sub>b s\<^sub>b \<Longrightarrow> 
+  orderly_code \<C>\<^sub>b 0 \<Longrightarrow> orderly_stack s\<^sub>b (length \<C>\<^sub>b) \<Longrightarrow> \<exists>\<Delta>\<^sub>b p s\<^sub>b'. s\<^sub>b = (\<Delta>\<^sub>b, Suc p) # s\<^sub>b' \<and> 
+    \<Delta>\<^sub>e = unflatten_values \<C>\<^sub>b \<Delta>\<^sub>b \<and> lookup \<C>\<^sub>b p = Some Return\<^sub>b \<and> s\<^sub>e = unflatten_stack \<C>\<^sub>b s\<^sub>b' \<and> \<C>\<^sub>e = []"
+proof (induction s\<^sub>b "length \<C>\<^sub>b" rule: orderly_stack.induct)
+  case (3 \<Delta>\<^sub>b p s\<^sub>b')
+  hence "Return\<^sub>e # \<C>\<^sub>e = unflatten_code \<C>\<^sub>b (Suc p) \<and> orderly_code \<C>\<^sub>b 0 \<and> p < length \<C>\<^sub>b" by simp
+  hence "lookup \<C>\<^sub>b p = Some Return\<^sub>b \<and> \<C>\<^sub>e = []" by blast
+  with 3 show ?case by simp
+qed simp_all
+
+lemma unflatten_stack_to_jump [dest]: "(\<Delta>\<^sub>e, Jump\<^sub>e # \<C>\<^sub>e) # s\<^sub>e = unflatten_stack \<C>\<^sub>b s\<^sub>b \<Longrightarrow> 
+  orderly_code \<C>\<^sub>b 0 \<Longrightarrow> orderly_stack s\<^sub>b (length \<C>\<^sub>b) \<Longrightarrow> \<exists>\<Delta>\<^sub>b p s\<^sub>b'. s\<^sub>b = (\<Delta>\<^sub>b, Suc p) # s\<^sub>b' \<and> 
+    \<Delta>\<^sub>e = unflatten_values \<C>\<^sub>b \<Delta>\<^sub>b \<and> lookup \<C>\<^sub>b p = Some Jump\<^sub>b \<and> s\<^sub>e = unflatten_stack \<C>\<^sub>b s\<^sub>b'"
+proof (induction s\<^sub>b "length \<C>\<^sub>b" rule: orderly_stack.induct)
+  case (3 \<Delta>\<^sub>b p s\<^sub>b')
+  hence "Jump\<^sub>e # \<C>\<^sub>e = unflatten_code \<C>\<^sub>b (Suc p) \<and> orderly_code \<C>\<^sub>b 0 \<and> p < length \<C>\<^sub>b" by simp
+  hence "lookup \<C>\<^sub>b p = Some Jump\<^sub>b \<and> \<C>\<^sub>e = []" by blast
+  with 3 show ?case by simp
+qed simp_all
+
+lemma unflatten_to_lam [dest]: "Lam\<^sub>e \<Delta>\<^sub>e \<C>\<^sub>e = unflatten_closure \<C>\<^sub>b v\<^sub>b \<Longrightarrow> 
+    \<exists>\<Delta>\<^sub>b p. v\<^sub>b = Lam\<^sub>b \<Delta>\<^sub>b p \<and> \<Delta>\<^sub>e = unflatten_values \<C>\<^sub>b \<Delta>\<^sub>b \<and> \<C>\<^sub>e = unflatten_code \<C>\<^sub>b p"
+  by (induction v\<^sub>b) simp_all
+
+lemma unflatten_state [dest]: "S\<^sub>e \<V>\<^sub>e s\<^sub>e = unflatten_state \<C> \<Sigma>\<^sub>b \<Longrightarrow> \<exists>\<V>\<^sub>b s\<^sub>b. 
+    \<Sigma>\<^sub>b = S\<^sub>b \<V>\<^sub>b s\<^sub>b \<and> \<V>\<^sub>e = unflatten_values \<C> \<V>\<^sub>b \<and> s\<^sub>e = unflatten_stack \<C> s\<^sub>b"
+  by (induction \<Sigma>\<^sub>b) simp_all
+
+theorem correct\<^sub>b [simp]: "unflatten_state \<C>\<^sub>b \<Sigma>\<^sub>b \<leadsto>\<^sub>e \<Sigma>\<^sub>e' \<Longrightarrow> orderly_state \<C>\<^sub>b \<Sigma>\<^sub>b \<Longrightarrow>
+  \<exists>\<Sigma>\<^sub>b'. iter (\<tturnstile> \<C>\<^sub>b \<leadsto>\<^sub>b) \<Sigma>\<^sub>b \<Sigma>\<^sub>b' \<and> unflatten_state \<C>\<^sub>b \<Sigma>\<^sub>b' = \<Sigma>\<^sub>e'"
+proof (induction "unflatten_state \<C>\<^sub>b \<Sigma>\<^sub>b" \<Sigma>\<^sub>e' rule: eval\<^sub>e.induct)
+  case (ev\<^sub>e_lookup \<Delta>\<^sub>e x v \<V>\<^sub>e \<C>\<^sub>e s\<^sub>e)
+  then obtain \<V>\<^sub>b s\<^sub>b where B: "\<Sigma>\<^sub>b = S\<^sub>b \<V>\<^sub>b s\<^sub>b \<and> \<V>\<^sub>e = unflatten_values \<C>\<^sub>b \<V>\<^sub>b \<and> 
+    (\<Delta>\<^sub>e, Lookup\<^sub>e x # \<C>\<^sub>e) # s\<^sub>e = unflatten_stack \<C>\<^sub>b s\<^sub>b" by fastforce
+  with ev\<^sub>e_lookup have "orderly_code \<C>\<^sub>b 0 \<and> orderly_stack s\<^sub>b (length \<C>\<^sub>b)" by simp
+  with B obtain \<Delta>\<^sub>b p s\<^sub>b' where S: "s\<^sub>b = (\<Delta>\<^sub>b, Suc p) # s\<^sub>b' \<and> 
+    \<Delta>\<^sub>e = unflatten_values \<C>\<^sub>b \<Delta>\<^sub>b \<and> lookup \<C>\<^sub>b p = Some (Lookup\<^sub>b x) \<and> \<C>\<^sub>e = unflatten_code \<C>\<^sub>b p \<and> 
+      s\<^sub>e = unflatten_stack \<C>\<^sub>b s\<^sub>b'" by (metis unflatten_stack_to_lookup)
+  with ev\<^sub>e_lookup obtain v' where V: "lookup \<Delta>\<^sub>b x = Some v' \<and> unflatten_closure \<C>\<^sub>b v' = v"
     by fastforce
-  moreover with iter_step have "orderly_state cd\<^sub>b \<Sigma>\<^sub>b'" by fastforce
-  ultimately obtain \<Sigma>\<^sub>b'' where "iter (\<tturnstile> cd\<^sub>b \<leadsto>\<^sub>b) \<Sigma>\<^sub>b' \<Sigma>\<^sub>b'' \<and> unflatten_state cd\<^sub>b \<Sigma>\<^sub>b'' = \<Sigma>\<^sub>t''" 
+  with S have "\<C>\<^sub>b \<tturnstile> S\<^sub>b \<V>\<^sub>b ((\<Delta>\<^sub>b, Suc p) # s\<^sub>b') \<leadsto>\<^sub>b S\<^sub>b (v' # \<V>\<^sub>b) ((\<Delta>\<^sub>b, p) # s\<^sub>b')" by simp
+  hence "iter (\<tturnstile> \<C>\<^sub>b \<leadsto>\<^sub>b) (S\<^sub>b \<V>\<^sub>b ((\<Delta>\<^sub>b, Suc p) # s\<^sub>b')) (S\<^sub>b (v' # \<V>\<^sub>b) ((\<Delta>\<^sub>b, p) # s\<^sub>b'))" by simp
+  with B S V show ?case by fastforce
+next
+  case (ev\<^sub>e_pushcon \<V>\<^sub>e \<Delta>\<^sub>e n \<C>\<^sub>e s\<^sub>e)
+  then obtain \<V>\<^sub>b s\<^sub>b where B: "\<Sigma>\<^sub>b = S\<^sub>b \<V>\<^sub>b s\<^sub>b \<and> \<V>\<^sub>e = unflatten_values \<C>\<^sub>b \<V>\<^sub>b \<and> 
+    (\<Delta>\<^sub>e, PushCon\<^sub>e n # \<C>\<^sub>e) # s\<^sub>e = unflatten_stack \<C>\<^sub>b s\<^sub>b" by fastforce
+  with ev\<^sub>e_pushcon have "orderly_code \<C>\<^sub>b 0 \<and> orderly_stack s\<^sub>b (length \<C>\<^sub>b)" by simp
+  with B obtain \<Delta>\<^sub>b p s\<^sub>b' where S: "s\<^sub>b = (\<Delta>\<^sub>b, Suc p) # s\<^sub>b' \<and> 
+    \<Delta>\<^sub>e = unflatten_values \<C>\<^sub>b \<Delta>\<^sub>b \<and> lookup \<C>\<^sub>b p = Some (PushCon\<^sub>b n) \<and> \<C>\<^sub>e = unflatten_code \<C>\<^sub>b p \<and> 
+      s\<^sub>e = unflatten_stack \<C>\<^sub>b s\<^sub>b'" by (metis unflatten_stack_to_pushcon)
+  with S have "\<C>\<^sub>b \<tturnstile> S\<^sub>b \<V>\<^sub>b ((\<Delta>\<^sub>b, Suc p) # s\<^sub>b') \<leadsto>\<^sub>b S\<^sub>b (Const\<^sub>b n # \<V>\<^sub>b) ((\<Delta>\<^sub>b, p) # s\<^sub>b')" by simp
+  hence "iter (\<tturnstile> \<C>\<^sub>b \<leadsto>\<^sub>b) (S\<^sub>b \<V>\<^sub>b ((\<Delta>\<^sub>b, Suc p) # s\<^sub>b')) (S\<^sub>b (Const\<^sub>b n # \<V>\<^sub>b) ((\<Delta>\<^sub>b, p) # s\<^sub>b'))" by simp
+  with B S show ?case by fastforce
+next
+  case (ev\<^sub>e_pushlam \<V>\<^sub>e \<Delta>\<^sub>e \<C>\<^sub>e' \<C>\<^sub>e s\<^sub>e)
+  then obtain \<V>\<^sub>b s\<^sub>b where B: "\<Sigma>\<^sub>b = S\<^sub>b \<V>\<^sub>b s\<^sub>b \<and> \<V>\<^sub>e = unflatten_values \<C>\<^sub>b \<V>\<^sub>b \<and> 
+    (\<Delta>\<^sub>e, PushLam\<^sub>e \<C>\<^sub>e' # \<C>\<^sub>e) # s\<^sub>e = unflatten_stack \<C>\<^sub>b s\<^sub>b" by fastforce
+  with ev\<^sub>e_pushlam have "orderly_code \<C>\<^sub>b 0 \<and> orderly_stack s\<^sub>b (length \<C>\<^sub>b)" by simp
+  with B obtain \<Delta>\<^sub>b p s\<^sub>b' p' where S: "s\<^sub>b = (\<Delta>\<^sub>b, Suc p) # s\<^sub>b' \<and> 
+    \<Delta>\<^sub>e = unflatten_values \<C>\<^sub>b \<Delta>\<^sub>b \<and> lookup \<C>\<^sub>b p = Some (PushLam\<^sub>b p') \<and> \<C>\<^sub>e = unflatten_code \<C>\<^sub>b p \<and> 
+      s\<^sub>e = unflatten_stack \<C>\<^sub>b s\<^sub>b' \<and> \<C>\<^sub>e' = unflatten_code \<C>\<^sub>b p'" by (metis unflatten_stack_to_pushlam)
+  with S have "\<C>\<^sub>b \<tturnstile> S\<^sub>b \<V>\<^sub>b ((\<Delta>\<^sub>b, Suc p) # s\<^sub>b') \<leadsto>\<^sub>b S\<^sub>b (Lam\<^sub>b \<Delta>\<^sub>b p' # \<V>\<^sub>b) ((\<Delta>\<^sub>b, p) # s\<^sub>b')" by simp
+  hence "iter (\<tturnstile> \<C>\<^sub>b \<leadsto>\<^sub>b) (S\<^sub>b \<V>\<^sub>b ((\<Delta>\<^sub>b, Suc p) # s\<^sub>b')) (S\<^sub>b (Lam\<^sub>b \<Delta>\<^sub>b p' # \<V>\<^sub>b) ((\<Delta>\<^sub>b, p) # s\<^sub>b'))" by simp
+  with B S show ?case by fastforce
+next
+  case (ev\<^sub>e_apply v \<Delta>\<^sub>e' \<C>\<^sub>e' \<V>\<^sub>e \<Delta>\<^sub>e \<C>\<^sub>e s\<^sub>e)
+  then obtain \<V>\<^sub>b s\<^sub>b where B: "\<Sigma>\<^sub>b = S\<^sub>b \<V>\<^sub>b s\<^sub>b \<and> 
+    v # Lam\<^sub>e \<Delta>\<^sub>e' \<C>\<^sub>e' # \<V>\<^sub>e = unflatten_values \<C>\<^sub>b \<V>\<^sub>b \<and> (\<Delta>\<^sub>e, Apply\<^sub>e # \<C>\<^sub>e) # s\<^sub>e = unflatten_stack \<C>\<^sub>b s\<^sub>b" 
+      by fastforce
+  with ev\<^sub>e_apply have "orderly_code \<C>\<^sub>b 0 \<and> orderly_stack s\<^sub>b (length \<C>\<^sub>b)" by simp
+  with B obtain \<Delta>\<^sub>b p s\<^sub>b' where S: "s\<^sub>b = (\<Delta>\<^sub>b, Suc p) # s\<^sub>b' \<and> 
+    \<Delta>\<^sub>e = unflatten_values \<C>\<^sub>b \<Delta>\<^sub>b \<and> lookup \<C>\<^sub>b p = Some Apply\<^sub>b \<and> \<C>\<^sub>e = unflatten_code \<C>\<^sub>b p \<and> 
+      s\<^sub>e = unflatten_stack \<C>\<^sub>b s\<^sub>b'" by (metis unflatten_stack_to_apply)
+  from B obtain vb \<Delta>\<^sub>b' p' \<V>\<^sub>b' where V: "\<V>\<^sub>b = vb # Lam\<^sub>b \<Delta>\<^sub>b' p' # \<V>\<^sub>b' \<and> 
+    v = unflatten_closure \<C>\<^sub>b vb \<and> \<Delta>\<^sub>e' = unflatten_values \<C>\<^sub>b \<Delta>\<^sub>b' \<and> \<C>\<^sub>e' = unflatten_code \<C>\<^sub>b p' \<and>
+      \<V>\<^sub>e = unflatten_values \<C>\<^sub>b \<V>\<^sub>b'" by fastforce
+  from S have "\<C>\<^sub>b \<tturnstile> S\<^sub>b (vb # Lam\<^sub>b \<Delta>\<^sub>b' p' # \<V>\<^sub>b') ((\<Delta>\<^sub>b, Suc p) # s\<^sub>b') \<leadsto>\<^sub>b
+    S\<^sub>b \<V>\<^sub>b' ((vb # \<Delta>\<^sub>b', p') # (\<Delta>\<^sub>b, p) # s\<^sub>b')" by simp
+  hence "iter (\<tturnstile> \<C>\<^sub>b \<leadsto>\<^sub>b) (S\<^sub>b (vb # Lam\<^sub>b \<Delta>\<^sub>b' p' # \<V>\<^sub>b') ((\<Delta>\<^sub>b, Suc p) # s\<^sub>b')) 
+    (S\<^sub>b \<V>\<^sub>b' ((vb # \<Delta>\<^sub>b', p') # (\<Delta>\<^sub>b, p) # s\<^sub>b'))" by simp
+  with B S V show ?case by auto                                              
+next
+  case (ev\<^sub>e_return \<V>\<^sub>e \<Delta>\<^sub>e \<C>\<^sub>e s\<^sub>e)
+  then obtain \<V>\<^sub>b s\<^sub>b where B: "\<Sigma>\<^sub>b = S\<^sub>b \<V>\<^sub>b s\<^sub>b \<and> \<V>\<^sub>e = unflatten_values \<C>\<^sub>b \<V>\<^sub>b \<and> 
+    (\<Delta>\<^sub>e, Return\<^sub>e # \<C>\<^sub>e) # s\<^sub>e = unflatten_stack \<C>\<^sub>b s\<^sub>b" by fastforce
+  with ev\<^sub>e_return have "orderly_code \<C>\<^sub>b 0 \<and> orderly_stack s\<^sub>b (length \<C>\<^sub>b)" by simp
+  with B obtain \<Delta>\<^sub>b p s\<^sub>b' where S: "s\<^sub>b = (\<Delta>\<^sub>b, Suc p) # s\<^sub>b' \<and> 
+    \<Delta>\<^sub>e = unflatten_values \<C>\<^sub>b \<Delta>\<^sub>b \<and> lookup \<C>\<^sub>b p = Some Return\<^sub>b \<and> s\<^sub>e = unflatten_stack \<C>\<^sub>b s\<^sub>b'" 
+      by (metis unflatten_stack_to_return)
+  with S have "\<C>\<^sub>b \<tturnstile> S\<^sub>b \<V>\<^sub>b ((\<Delta>\<^sub>b, Suc p) # s\<^sub>b') \<leadsto>\<^sub>b S\<^sub>b \<V>\<^sub>b s\<^sub>b'" by simp
+  hence "iter (\<tturnstile> \<C>\<^sub>b \<leadsto>\<^sub>b) (S\<^sub>b \<V>\<^sub>b ((\<Delta>\<^sub>b, Suc p) # s\<^sub>b')) (S\<^sub>b \<V>\<^sub>b s\<^sub>b')" by simp
+  with B S show ?case by fastforce
+next
+  case (ev\<^sub>e_jump v \<Delta>\<^sub>e' \<C>\<^sub>e' \<V>\<^sub>e \<Delta>\<^sub>e \<C>\<^sub>e s\<^sub>e)
+  then obtain \<V>\<^sub>b s\<^sub>b where B: "\<Sigma>\<^sub>b = S\<^sub>b \<V>\<^sub>b s\<^sub>b \<and> 
+    v # Lam\<^sub>e \<Delta>\<^sub>e' \<C>\<^sub>e' # \<V>\<^sub>e = unflatten_values \<C>\<^sub>b \<V>\<^sub>b \<and> 
+      (\<Delta>\<^sub>e, Jump\<^sub>e # \<C>\<^sub>e) # s\<^sub>e = unflatten_stack \<C>\<^sub>b s\<^sub>b" by fastforce
+  with ev\<^sub>e_jump have "orderly_code \<C>\<^sub>b 0 \<and> orderly_stack s\<^sub>b (length \<C>\<^sub>b)" by simp
+  with B obtain \<Delta>\<^sub>b p s\<^sub>b' where S: "s\<^sub>b = (\<Delta>\<^sub>b, Suc p) # s\<^sub>b' \<and> 
+    \<Delta>\<^sub>e = unflatten_values \<C>\<^sub>b \<Delta>\<^sub>b \<and> lookup \<C>\<^sub>b p = Some Jump\<^sub>b \<and> s\<^sub>e = unflatten_stack \<C>\<^sub>b s\<^sub>b'" 
+      by (metis unflatten_stack_to_jump)
+  from B obtain vb \<Delta>\<^sub>b' p' \<V>\<^sub>b' where V: "\<V>\<^sub>b = vb # Lam\<^sub>b \<Delta>\<^sub>b' p' # \<V>\<^sub>b' \<and> 
+    v = unflatten_closure \<C>\<^sub>b vb \<and> \<Delta>\<^sub>e' = unflatten_values \<C>\<^sub>b \<Delta>\<^sub>b' \<and> \<C>\<^sub>e' = unflatten_code \<C>\<^sub>b p' \<and>
+      \<V>\<^sub>e = unflatten_values \<C>\<^sub>b \<V>\<^sub>b'" by fastforce
+  from S have "\<C>\<^sub>b \<tturnstile> S\<^sub>b (vb # Lam\<^sub>b \<Delta>\<^sub>b' p' # \<V>\<^sub>b') ((\<Delta>\<^sub>b, Suc p) # s\<^sub>b') \<leadsto>\<^sub>b
+    S\<^sub>b \<V>\<^sub>b' ((vb # \<Delta>\<^sub>b', p') # s\<^sub>b')" by simp
+  hence "iter (\<tturnstile> \<C>\<^sub>b \<leadsto>\<^sub>b) (S\<^sub>b (vb # Lam\<^sub>b \<Delta>\<^sub>b' p' # \<V>\<^sub>b') ((\<Delta>\<^sub>b, Suc p) # s\<^sub>b')) 
+    (S\<^sub>b \<V>\<^sub>b' ((vb # \<Delta>\<^sub>b', p') # s\<^sub>b'))" by simp
+  with B S V show ?case by auto                                              
+qed
+
+lemma iter_correct\<^sub>b [simp]: "iter (\<leadsto>\<^sub>e) (unflatten_state \<C>\<^sub>b \<Sigma>\<^sub>b) \<Sigma>\<^sub>e' \<Longrightarrow> orderly_state \<C>\<^sub>b \<Sigma>\<^sub>b \<Longrightarrow>
+  \<exists>\<Sigma>\<^sub>b'. iter (\<tturnstile> \<C>\<^sub>b \<leadsto>\<^sub>b) \<Sigma>\<^sub>b \<Sigma>\<^sub>b' \<and> unflatten_state \<C>\<^sub>b \<Sigma>\<^sub>b' = \<Sigma>\<^sub>e'"
+proof (induction "unflatten_state \<C>\<^sub>b \<Sigma>\<^sub>b" \<Sigma>\<^sub>e' arbitrary: \<Sigma>\<^sub>b rule: iter.induct)
+  case (iter_step \<Sigma>\<^sub>e' \<Sigma>\<^sub>e'')
+  moreover then obtain \<Sigma>\<^sub>b' where S: "iter (\<tturnstile> \<C>\<^sub>b \<leadsto>\<^sub>b) \<Sigma>\<^sub>b \<Sigma>\<^sub>b' \<and> unflatten_state \<C>\<^sub>b \<Sigma>\<^sub>b' = \<Sigma>\<^sub>e'" 
+    by fastforce
+  moreover with iter_step have "orderly_state \<C>\<^sub>b \<Sigma>\<^sub>b'" by fastforce
+  ultimately obtain \<Sigma>\<^sub>b'' where "iter (\<tturnstile> \<C>\<^sub>b \<leadsto>\<^sub>b) \<Sigma>\<^sub>b' \<Sigma>\<^sub>b'' \<and> unflatten_state \<C>\<^sub>b \<Sigma>\<^sub>b'' = \<Sigma>\<^sub>e''" 
     by fastforce
   with S show ?case by (metis iter_append)
 qed force+
 
-lemma unfl_terminal [simp]: "unflatten_state cd \<Sigma> = S\<^sub>e [c] [] \<Longrightarrow>
-  \<exists>v. \<Sigma> = S\<^sub>b [v] [] \<and> c = unflatten_closure cd v"
+lemma unfl_terminal [simp]: "unflatten_state \<C>\<^sub>b \<Sigma> = S\<^sub>e [c] [] \<Longrightarrow>
+  \<exists>v. \<Sigma> = S\<^sub>b [v] [] \<and> c = unflatten_closure \<C>\<^sub>b v"
 proof -
-  assume "unflatten_state cd \<Sigma> = S\<^sub>e [c] []"
-  then obtain vs sfs where S: "\<Sigma> = S\<^sub>b vs sfs \<and> [c] = unflatten_values cd vs \<and> [] = unflatten_stack cd sfs" 
-    by (metis unfl_state)
-  moreover then obtain v where "vs = [v] \<and> c = unflatten_closure cd v" by blast
+  assume "unflatten_state \<C>\<^sub>b \<Sigma> = S\<^sub>e [c] []"
+  then obtain \<V>\<^sub>b s where S: "\<Sigma> = S\<^sub>b \<V>\<^sub>b s \<and> [c] = unflatten_values \<C>\<^sub>b \<V>\<^sub>b \<and> [] = unflatten_stack \<C>\<^sub>b s" 
+    by (metis unflatten_state)
+  moreover then obtain v where "\<V>\<^sub>b = [v] \<and> c = unflatten_closure \<C>\<^sub>b v" by blast
   ultimately show ?thesis by simp
 qed
 
-lemma evalb_end [simp]: "iter (\<leadsto>\<^sub>e) (unflatten_state cd\<^sub>b \<Sigma>\<^sub>b) (S\<^sub>e [c] []) \<Longrightarrow> 
-  orderly_state cd\<^sub>b \<Sigma>\<^sub>b \<Longrightarrow> 
-    \<exists>v. iter (\<tturnstile> cd\<^sub>b \<leadsto>\<^sub>b) \<Sigma>\<^sub>b (S\<^sub>b [v] []) \<and> c = unflatten_closure cd\<^sub>b v"
+lemma eval\<^sub>b_end [simp]: "iter (\<leadsto>\<^sub>e) (unflatten_state \<C>\<^sub>b \<Sigma>\<^sub>b) (S\<^sub>e [c] []) \<Longrightarrow> 
+  orderly_state \<C>\<^sub>b \<Sigma>\<^sub>b \<Longrightarrow> 
+    \<exists>v. iter (\<tturnstile> \<C>\<^sub>b \<leadsto>\<^sub>b) \<Sigma>\<^sub>b (S\<^sub>b [v] []) \<and> c = unflatten_closure \<C>\<^sub>b v"
 proof -
-  assume "iter (\<leadsto>\<^sub>e) (unflatten_state cd\<^sub>b \<Sigma>\<^sub>b) (S\<^sub>e [c] [])"
-  moreover assume O: "orderly_state cd\<^sub>b \<Sigma>\<^sub>b"
-  ultimately obtain \<Sigma>\<^sub>b' where E: "iter (\<tturnstile> cd\<^sub>b \<leadsto>\<^sub>b) \<Sigma>\<^sub>b \<Sigma>\<^sub>b' \<and> unflatten_state cd\<^sub>b \<Sigma>\<^sub>b' = S\<^sub>e [c] []" 
+  assume "iter (\<leadsto>\<^sub>e) (unflatten_state \<C>\<^sub>b \<Sigma>\<^sub>b) (S\<^sub>e [c] [])"
+  moreover assume O: "orderly_state \<C>\<^sub>b \<Sigma>\<^sub>b"
+  ultimately obtain \<Sigma>\<^sub>b' where E: "iter (\<tturnstile> \<C>\<^sub>b \<leadsto>\<^sub>b) \<Sigma>\<^sub>b \<Sigma>\<^sub>b' \<and> unflatten_state \<C>\<^sub>b \<Sigma>\<^sub>b' = S\<^sub>e [c] []" 
     by fastforce
-  moreover with O have "orderly_state cd\<^sub>b \<Sigma>\<^sub>b'" by fastforce
-  moreover with E obtain v where "\<Sigma>\<^sub>b' = S\<^sub>b [v] [] \<and> c = unflatten_closure cd\<^sub>b v" 
+  moreover with O have "orderly_state \<C>\<^sub>b \<Sigma>\<^sub>b'" by fastforce
+  moreover with E obtain v where "\<Sigma>\<^sub>b' = S\<^sub>b [v] [] \<and> c = unflatten_closure \<C>\<^sub>b v" 
     by (metis unfl_terminal)
   ultimately show ?thesis by blast
 qed
